Moving the generic stuff to Env.v Working on Expr, not complete yet.

src/Expr.v
@@ -1,511 +1,493 @@
-(** TODO List
- ** - Merging states
- ** - Lifting expressions to new states
- ** - Prover for simple domain
- ** - Unification variables?
- ** - Expression equality
- **)
+Require Import List Eqdep_dec.
+Require Import Env.
 
-Require Import String.
-Require Import List Arith.
+Set Implicit Arguments.
 
-Set Implicit Arugments.
-Set Strict Implicit.
+Section env.
+  Record type := {
+    Impl : Type;
+    Eq : forall x y : Impl, option (x = y)
+  }.
 
-Section FunType.
-  Context {T U : Type}.
-  Variable D : T -> Type.
-  Variable R : U -> Type.
+  Variable types : list type.
 
-  Fixpoint funtype (ls : list T) (r : U) : Type :=
-    match ls with 
-      | nil => R r
-      | a :: b => D a -> funtype b r
+  Definition tvar := option (fin (length types)).
+  Definition tvarD x := match x with
+                          | None => Prop
+                          | Some x => Impl (get types x)
+                        end.
+
+  Fixpoint functionTypeD (domain : list tvar) (range : tvar) : Type :=
+    match domain with
+      | nil => tvarD range
+      | d :: domain' => tvarD d -> functionTypeD domain' range
     end.
 
-  Definition funtype' (x : list T * U) : Type :=
-    match x with
-      | (x,y) => funtype x y
-    end.
-End FunType.
+  Record signature := {
+    Domain : list tvar;
+    Range : tvar;
+    Denotation : functionTypeD Domain Range
+  }.
 
-Section Member.
-  Context {T : Type}. 
+  Definition functions := list signature.
+  Definition variables := list tvar.
 
-  Inductive Mem (V : T) : list T -> Type :=
-  | MHere : forall R, Mem V (V :: R)
-  | MNext : forall V' R, Mem V R -> Mem V (V' :: R).
+  Variable funcs : functions.
+  Variable vars : variables.
 
-  Variable D : T -> Type.
+  Definition func := fin (length funcs).
+  Definition var := fin (length vars).
 
-  Fixpoint Env (g : list T) : Type :=
-    match g with
-      | nil => unit
-      | a :: b => D a * Env b
-    end%type.
+  Inductive expr : tvar -> Type :=
+  | Const : forall t : tvar, tvarD t -> expr t
+  | Var : forall x : var, expr (get vars x)
+  | Func : forall f : func, hlist expr (Domain (get funcs f)) -> expr (Range (get funcs f)).
 
-  Fixpoint Env_app {s s' : list T} : Env s -> Env s' -> Env (s ++ s') :=
-    match s with 
-      | nil => fun _ x => x
-      | a :: b => fun l r => 
-        (fst l, Env_app (snd l) r)
-    end.
+  Section applyD.
+    Variable exprD : forall t, expr t -> tvarD t.
 
-  Fixpoint get {t} (s : list T) (m : Mem t s) : Env s -> D t :=
-    match m with
-      | MHere _ => fun x => fst x
-      | MNext _ _ r => fun x => get _ r (snd x)
-    end.
+    Fixpoint applyD domain (xs : hlist expr domain)
+      : forall range, functionTypeD domain range -> tvarD range :=
+        match xs in hlist _ domain return forall range, functionTypeD domain range -> tvarD range with
+          | HNil => fun _ x => x
+          | HCons _ _ x xs' => fun _ f => applyD xs' _ (f (exprD x))
+        end.
+  End applyD.
 
-  Fixpoint lift {V} ls lse : Mem V ls -> Mem V (lse ++ ls) :=
-    match lse with 
-      | nil => fun x => x 
-      | a :: b => fun x => MNext _ _ _ (lift ls b x)
-    end.
+  Variable env : hlist tvarD vars.
 
-  Fixpoint extend {V} ls lse (m : Mem V ls) : Mem V (ls ++ lse) :=
-    match m with 
-      | MHere x => MHere V (x ++ lse)
-      | MNext _ R m => MNext V _ (R ++ lse) (extend R lse m)
-    end.
-
-  Require Import Program.
-
-  Fixpoint count {V ls} (m : Mem V ls) : nat :=
-    match m with
-      | MHere _ => 0
-      | MNext _ _ m => 1 + count m
+  Fixpoint exprD t (e : expr t) {struct e} : tvarD t :=
+    match e with
+      | Const _ c => c
+      | Var x => hlist_get x env
+      | Func f xs => applyD exprD xs _ (Denotation (get funcs f))
     end.
   
-  Theorem eq_if_count : forall V ls (l r : Mem V ls), 
-    count l = count r -> l = r.
-  Proof.
-    induction l; dependent destruction r; simpl in *; intros; try congruence; auto.
-    inversion H. eapply IHl in H1. subst; reflexivity.
-  Qed.
+  Lemma tvar_dec : forall (a b : tvar), {a = b} + {a <> b}.
+    decide equality. eapply finEq. 
+  Defined.
 
-  Theorem neq_if_ncount : forall V ls (l r : Mem V ls), 
-    count l <> count r -> l <> r.
-  Proof.
-    induction l; dependent destruction r; simpl in *; intros; try congruence; auto.
-    intro. inversion H0. intro. inversion H0.
-    Require Import EqdepFacts.
-    intro. apply H. inversion H0. eapply inj_pair2 in H2. subst; reflexivity.
-  Qed.
+  Definition exprEq : forall t (x y : expr t), option (x = y).
+  refine (fix exprEq t (x : expr t) {struct x} : forall y : expr t, option (x = y) :=
+    match x in expr t return forall y : expr t, option (x = y) with
+      | Const t c1 => fun y : expr t => match y in expr t' return forall c1 : tvarD t', option (Const t' c1 = y) with
+                                          | Const t c2 => match t return forall c2 c1 : tvarD t, option (Const t c1 = Const t c2) with
+                                                            | None => fun _ _ => None
+                                                            | Some t => fun x y => if Eq (get types t) x y then Some _ else None
+                                                          end c2
+                                          | _ => fun _ => None
+                                        end c1
+      | Var x1 => fun y => 
+        match y in expr t return forall Heq : t = get vars x1, option (Var x1 = match Heq in _ = T return expr T with
+                                                                                            | refl_equal => y
+                                                                                          end) with
+                             | Var x2 => fun Heq => if finEq x1 x2 then Some _ else None
+                             | _ => fun _ => None
+                           end (refl_equal _)
+      | Func f1 xs1 => fun y => match y in expr t return forall Heq : t = Range (get funcs f1),
+                                    (forall xs2, option (xs1 = xs2))
+                                    -> option (Func f1 xs1 = match Heq in _ = T return expr T with
+                                                               | refl_equal => y
+                                                             end) with
+                                    | Func f2 xs2 => fun Heq cmp => match finEq f1 f2 with
+                                                                      | right _ => None
+                                                                      | left Heq' =>
+                                                                        if cmp (match sym_eq Heq' in _ = F
+                                                                                  return hlist expr (Domain (get funcs F)) with
+                                                                                  | refl_equal => xs2
+                                                                                end) then Some _ else None
+                                                                    end
+                                    | _ => fun _ _ => None
+                                  end (refl_equal _) (hlistEq exprEq xs1)
+      end); clear exprEq; try abstract (subst;
+        repeat match goal with
+                 | [ Heq : _ = _ |- _ ] => rewrite (UIP_dec tvar_dec Heq (refl_equal _)) in *; clear Heq; simpl in *
+               end; congruence).
+  Defined.
+End env.
 
+Section Qexpr.
+  Context {types : list type}.
+  Variable fs : functions types.
 
-  Definition eqMem {V ls} (l r : Mem V ls) : {l = r} + {l <> r} :=
-    match eq_nat_dec (count l) (count r) with 
-      | left pf => left _ (eq_if_count _ _ _ _ pf) 
-      | right pf => right _ (neq_if_ncount _ _ _ _ pf)
-    end.
+  Definition Qexpr := { x : variables types & expr fs x None }.
 
-End Member.
-
-Notation "'$>' a" := (@MNext _ _ _ _ a) (at level 5).
-Notation "'$$'" := (@MHere _ _ _) (at level 5).
-
-(** Reflection State **)
-Fixpoint List2Fun (D : Type) (ls : list Type) (n : nat) : nat -> Type :=
-  match ls with
-    | nil => fun _ => D
-    | a :: b => 
-      let r := List2Fun D b (S n) in
-      fun x => if eq_nat_dec x n then a else r x
-  end.
-
-Definition maybe {T U : Type} (D : T) (F : U -> T) (o : option U) : T :=
-  match o with
-    | None => D
-    | Some t => F t
-  end.
-
-Record ReflSpine : Type :=
-{ Typs        : list Type
-; constsOf    : nat -> Type
-; Sym_type    : list (list nat * option nat)
-}.
-
-Inductive empty : Type := .
-
-Record ReflDenote (RS : ReflSpine) : Type :=
-{ Typ_denote  := List2Fun empty (Typs RS) 0
-; constIn     : forall T, constsOf RS T -> Typ_denote T
-; Sym_denote  : Env (funtype' Typ_denote (maybe Prop Typ_denote)) (Sym_type RS)
-}.
-
-Implicit Arguments Typ_denote [ RS ].
-Implicit Arguments constIn [ RS ].
-Implicit Arguments Sym_denote [ RS ].
-
-(** Syntax of Expressions **)
-Section Expr.
-  Variable RS : ReflSpine.
-  Variable RD : ReflDenote RS.
-  Variable vs : list nat.
-  Variable VE : Env (Typ_denote RD) vs.
-
-  Inductive Expr : option nat -> Type := 
-    (** variables **)
-  | Var  : forall T, Mem T vs -> Expr (Some T)
-    (** functions **)
-  | App : forall Ts T, Mem (Ts,T) (Sym_type RS) -> Exprs Ts -> Expr T
-    (** constants **)
-  | Const : forall T, constsOf RS T -> Expr (Some T)
-  with Exprs : list nat -> Type :=
-  | Enil  : Exprs nil
-  | Econs : forall T Ts, Expr (Some T) -> Exprs Ts -> Exprs (T :: Ts)
-  .
-
-  (** TODO : Expr Equality **)
-
-  Fixpoint denoteExpr T (e : Expr T) : maybe Prop (Typ_denote RD) T :=
-    match e in Expr T return maybe Prop (Typ_denote RD) T with 
-      | Var _ m => get _ _ m VE
-      | App Ts T s es =>
-        denoteExprs Ts T es (get (funtype' (Typ_denote RD) (maybe Prop (Typ_denote RD))) (Sym_type RS) s (Sym_denote RD))
-      | Const _ x => constIn RD _ x 
-    end
-  with denoteExprs Ts T (es : Exprs Ts) 
-    : funtype (Typ_denote RD) (maybe Prop (Typ_denote RD)) Ts T -> maybe Prop (Typ_denote RD) T :=
-    match es with 
-      | Enil => fun r => r
-      | Econs _ _ x y => fun f => denoteExprs _ _ y (f (denoteExpr _ x))
-    end.
-
-End Expr.
-
-Implicit Arguments App [ RS Ts T ].
-Implicit Arguments Const [ RS T ].
-Implicit Arguments Var [ RS T ].
-Implicit Arguments denoteExpr [ RS vs ].
-Implicit Arguments denoteExprs [ RS vs ].
-
-(*
-Section Lifting.
-  Context {Typ : Type}. 
-  Variable constsOf : Typ -> Type.
-  Variable (ss sse : list (list Typ * option Typ)).
-  Variable (vs ve : list Typ).
-
-  Fixpoint liftExpr T (e : Expr constsOf ss vs T) : Expr constsOf (sse ++ ss) (ve ++ vs) T :=
-    match e with
-      | App Ts T s es =>
-        let es' := liftExprs Ts es in
-        App constsOf (sse ++ ss) (ve ++ vs) Ts T (lift ss sse s) es'
-      | Const a b => Const constsOf _ _ a b
-      | Var _ m => Var _ _ _ _ (lift vs ve m)  
-    end
-  with liftExprs Ts (es : Exprs constsOf ss vs Ts) : Exprs constsOf (sse ++ ss) (ve ++ vs) Ts :=
-    match es with
-      | Enil => Enil constsOf (sse ++ ss) (ve ++ vs)
-      | Econs _ _ x y => Econs constsOf _ _ _ _ (liftExpr _ x) (liftExprs _ y)
-    end.
-    
-End Lifting.
-*)
-
-Section QExpr.
-  Variable RS : ReflSpine.
-
-  Definition QExpr := 
-    { x : list nat & Expr RS x None }.
-
-  Variable RD : ReflDenote RS.
-
-  Fixpoint denoteQuant (ls : list nat) : (Env (Typ_denote RD) ls -> Prop) -> Prop :=
-    match ls with
-      | nil => fun cc => cc tt
+  Fixpoint denoteQuant (ls : variables types) : (hlist (tvarD types) ls -> Prop) -> Prop :=
+    match ls as ls return (hlist (tvarD types) ls -> Prop) -> Prop with
+      | nil => fun cc => cc (HNil)
       | a :: b => fun cc => 
-        forall (x : Typ_denote RD a), denoteQuant b (fun g => cc (x, g))
+        forall x, denoteQuant (fun g => cc (HCons x g))
     end.
 
-  Definition denoteQExpr (p : QExpr) : Prop :=
-    denoteQuant (projT1 p) 
-      (fun x : Env (Typ_denote RD) (projT1 p) => denoteExpr RD x None (projT2 p)).
-End QExpr.
+  Definition qexprD (p : Qexpr) : Prop :=
+    @denoteQuant (projT1 p) (fun x => exprD x (projT2 p)).
+End Qexpr.
+
+Section ProverT.
+  Context {types : list type}.
+  Context {fs : functions types}.
+
+  Definition ProverT : Type := forall 
+    (hyps : list (@Qexpr types fs))
+    (goal : @expr types fs nil None), 
+    hlist (@qexprD _ fs) hyps -> option (exprD HNil goal).
 
 (*
-Definition extendReflState (a b : ReflState) : ReflState :=
-  let atyp_count := length (Typs a) in
-  {| Typs     := Typs a ++ Typs b
-   ; constsOf := fun x => if lt_dec x atyp_count then constsOf x else 
+  Definition unify (T : type) (e1 e2 : expr fs vs T) : option (expr fs )
 *)
 
-(* TODO : This type is a mess 
-Definition ProverT (RS : ReflState) :=
-  forall Typ_ext SymT_ext 
-    (SymD_ext : Env (funtype' (List2Fun (Typs RS ++ Typ_ext) 0) (Typ_denote' (List2Fun (Typs RS ++ Typ_ext) 0))) (Sym_type RS ++ SymT_ext))
-    (Hs : list (QExpr (constsOf RS) (Sym_type RS ++ SymT_ext))),
-    Env (denoteQExpr (constsOf RS) (List2Fun (Typs RS ++ Typ_ext) 0) (constIn RS) (Sym_type RS ++ SymT_ext) (Env_app _ (Sym_denote RS) SymD_ext)) Hs -> 
-    forall (G : Expr (constsOf RS) (Sym_type RS ++ SymT_ext) nil None),
-      option (denoteExpr _ (Sym_type RS ++ SymT_ext) nil (Typ_denote RS) (constIn RS) (Env_app _ (Sym_denote RS) SymD_ext) tt None G).
 
+  Definition assumptionProver : ProverT.
+    unfold ProverT.
+    refine (fix assumptionProver hyps (goal : expr fs nil None) : hlist (@qexprD _ fs) hyps -> option (exprD HNil goal) :=
+      match hyps with
+        | nil => fun _ => None
+        | existT vs exp :: b => 
+          match vs as vs return forall exp : expr fs vs None, hlist (@qexprD _ fs) (existT (fun vs => expr fs vs None) vs exp :: b) -> _ with
+            | nil => fun exp pfHyps => if exprEq goal exp then Some _ else assumptionProver b goal (hlist_tl pfHyps)
+            | _ => fun _ pfHyps => assumptionProver b goal (hlist_tl pfHyps)
+          end exp
+      end).
+  generalize ((hlist_hd pfHyps)). unfold qexprD. simpl. rewrite _H. intro. apply H.
 
-Definition nat_prover : ProverT ReflState_nat. 
-Admitted.
-*)
+    (** TODO :
+        - How would I implement one of these? 
+        - Termination will be problematic...
+     **)
+  Defined.
+  
+End ProverT.
 
-Definition ReflSpine_nat : ReflSpine := Eval simpl in 
-  let typs := (nat:Type) :: @nil Type in
-  let constsOf := List2Fun empty typs 0 in (* fun x : nat => if eq_nat_dec x 0 then nat else empty in *)
-  {| Typs       := typs
-   ; constsOf   := constsOf
-   ; Sym_type   := (0 :: 0 :: nil, Some 0) :: (*0 :: 0 :: nil, None) ::*) nil
-   |}.
+Section PartialApply.
+  Fixpoint funtype (ls : list Type) (r : Type) : Type :=
+    match ls with 
+      | nil => r
+      | a :: b => a -> funtype b r
+    end.
 
-Definition ReflDenote_nat : ReflDenote ReflSpine_nat := 
-  let Typ_denote := List2Fun empty (Typs ReflSpine_nat) 0 in
-  {| constIn   := fun T => match T as T return constsOf ReflSpine_nat T  -> Typ_denote T with
-                             | 0 => fun x => x
-                             | _ => fun x => match x with
-                                             end
-                           end
-  ; Sym_denote := (plus, tt)
-  |}.
+  Fixpoint apply_ls (ls : list Type) (T : Type) (R : T -> Type) (V : T)
+    : funtype ls (forall x : T, R x) -> funtype ls (R V) :=
+    match ls with
+      | nil => fun F => F V
+      | a :: b => fun F => fun x : a => apply_ls b R V (F x)
+    end.
+End PartialApply.
 
-(**********************
- ** Reflecting Types **
- **********************)
-Ltac refl_type env i T :=
-  match env with
-    | T :: _ => constr:((i, env))
-    | ?X :: ?E =>
-      let n := constr:(S i) in
-      match refl_type E n T with
-        | ( ?I , ?E ) =>
-          constr:((X :: E, I))
-      end
-    | nil => constr:((i, T :: nil))
-  end.
-
-Ltac refl_ret_type Ts T :=
+Ltac extend_type T D types :=
   match T with
-    | Prop => None
-    | _ => match refl_type Ts 0 T with
-             | ( ?rT , _ ) => 
-               constr:(Some rT)
-           end
-  end.
-
-Ltac refl_fun_type env T :=
-  match T with
-    | Prop => 
-      constr:(((@nil nat , @None nat), env))
-    | ?T1 -> ?T2 => 
-      match refl_type env 0 T1 with
-        | ( ?t1 , ?env' ) => 
-          match refl_fun_type env' T2 with
-            | ( ( ?AS , ?RT ) , ?E ) => 
-              constr:(((t1 :: AS , RT), E))
+    | Prop => types
+    | _ => 
+      let rec find types :=
+      match types with
+        | nil => constr:(false)
+        | ?a :: ?b =>
+          let T' := eval simpl Impl in (Impl a) in
+          match T' with
+            | T => constr:(true)
+            | _ => find b
           end
       end
-    | _ => 
-      match refl_type env 0 T with
-        | ( ?I , ?E ) => 
-          constr:(((@nil nat, Some I), E))
-      end
+    in
+    match find types with
+      | true => types
+      | _ => constr:(D :: types)
+    end
   end.
 
-
-(** Ltac "lookup a symbol in an Env". fail if non-existant **)
-Ltac lookup x es ev :=
-  match ev with
-    | ( x , _ ) => 
-      match es with
-        | ?T :: ?TS =>
-          let r := constr:(@MHere _ T TS) in r
-      end
-    | ( _ , ?R ) =>
-      match es with
-        | ?T :: ?TS =>
-          let r := lookup x TS R in
-          constr:(@MNext _ _ T TS r)
-      end
-  end.
-
-Ltac lookup_cc fcc scc es ev x :=
-  match ev with
-    | ( x , _ ) => 
-      match es with
-        | ?T :: ?TS =>
-          let r := constr:(@MHere _ T TS) in scc r
-      end
-    | ( _ , ?R ) =>
-      match es with
-        | ?T :: ?TS =>
-          let scc' r := 
-            let k := constr:(@MNext _ _ T TS r) in scc k
-          in
-          lookup_cc fcc scc' TS R x
-      end
-    | tt => fcc x
-  end.
-
-
-Fixpoint apply_ls (ls : list Type) (T : Type) (R : T -> Type) (V : T)
-  : funtype (fun x => x) (fun _ => forall x, R x) ls tt -> funtype (fun x => x) (fun x => R V) ls tt :=
-  match ls with
-    | nil => fun F => F V
-    | a :: b => fun F => fun x : a => apply_ls b T R V (F x)
-  end.
+Definition defaultType T := {| Impl := T; Eq := fun _ _ => None |}.
 
 Ltac refl_app cc e := 
-  let aT := constr:(@nil Type) in
-  let rec refl e As :=
+  let rec refl cc e As :=
     match e with
       | ?A ?B =>
-        let As' := constr:((B, As)) in
-        refl A As' 
-      | _ => 
-        let T := type of e in
-        cc e aT T As
+        let Ta := type of A in
+        match type of A with
+          | _ -> ?TT => 
+            let As := constr:((B, As)) in
+            let Tb := type of B in
+            let cc f Ts args := 
+              let Ts' := constr:(Ts ++ (Tb : Type) :: nil) in
+              cc f Ts' args
+            in 
+            refl cc A As
+          | forall x : ?T1, @?T2 x => 
+            let cc f Ts args := 
+              let Tb  := type of B in
+              let f'  := eval simpl in (@apply_ls Ts T1 T2 B f) in
+              cc f' Ts args
+            in
+            refl cc A As
+        end
+      | _ =>
+        let Ts := constr:(@nil Type) in
+        cc e Ts As
     end
   in
   let b := constr:(tt) in
-  refl e b.
+  refl cc e b.
 
-Ltac reflect_expr refl_const RS Ts Ss Sv Vs Vv e :=
-  let aT := constr:(@nil Type) in
-  let rec refl_expr e :=
-    let app_case e :=
-      match refl_app reflect_args e with
-        | ( ?args , ?F ) =>
-          let m := lookup F Ss Sv in
-          constr:(@App RS Vs _ _ m args)
-      end        
-    in
-    let var_case m :=
-      constr:(Var RS Vs _ m)
-    in
-    let const_case m :=
-      let T := type of e in
-      match refl_type Ts 0 T with
-        | ( ?rT , _ ) =>  (** the second component should be equal to Ts **)
-          constr:(@Const RS Vs rT m)
-      end
-    in
-    let var_app_case := lookup_cc app_case var_case Vs Vv in
-    refl_const const_case var_app_case e 
-      
-  with reflect_args F Typs Ft As :=
-    match As with
-      | tt =>
-        constr:((Enil RS Vs, F))
-      | ( ?A , ?As ) => 
-        match Ft with
-          | ?T1 -> ?T2 => 
-            let Typs' := constr:(Typs ++ (T1:Type) :: @nil Type) in
-            match reflect_args F Typs' T2 As with
-              | ( ?res , ?F' ) => 
-                match refl_type Ts 0 T1 with
-                  | ( ?rT , _ ) =>
-                    let Ae := refl_expr A in
-                    constr:((Econs RS Vs rT _ Ae res , F'))
-                 end
-            end  
-          | forall x : ?T1 , @?T2 x => 
-            let Ft' := eval simpl in (T2 A) in
-            let Typs' := eval simpl app in Typs in
-            let F'' := eval simpl in (apply_ls Typs' T1 T2 A F) in
-            reflect_args F'' Typs' Ft' As
-        end
+Ltac extend_all_types Ts types :=
+  match Ts with
+    | nil => types
+    | ?a :: ?b => 
+      let types := extend_type a (defaultType a) types in
+      extend_all_types b types
+  end.
+
+Ltac buildTypes e types :=
+  let rec bt_args args types :=
+    match args with
+      | nil => types
+      | ?a :: ?b => 
+        let types := buildTypes a types in
+        bt_args b types
     end
   in
-  refl_expr e.
-
-(** lookup "x" in "Vs" (spine of Vs is given in Ts, denotation of Ts given in E) **)
-Ltac set_add Ts Ss Sv x :=
-  match Sv with
-    | ( x , _ ) => constr:((Ts, Ss, Sv))
-    | tt => 
-      let t := type of x in
-      match refl_fun_type Ts t with
-        | ( ?T , ?Ts ) =>
-          constr:((Ts, T :: nil, (x, tt)))
-      end
-    | ( ?V , ?Vs ) =>
-      match Ss with
-        | ?S :: ?Ss =>
-          match set_add Ts Ss Vs x with
-            | ( ?Ts , ?Ss , ?Vs ) => constr:((Ts , S :: Ss, (V, Vs)))
-          end
-      end
-  end.
-
-Ltac set_add' st x :=
-  match st with
-    | ( ?Ts , ?Ss , ?Sv ) => set_add Ts Ss Sv x
-  end.
-
-Ltac refl_nat_const scc fcc e := 
-  match e with
-    | 0   => scc e 
-    | S _ => scc e
-    | _ => fcc e
-  end.
-
-Ltac gather_symbols refl_const Ts Ss Sv exp :=
-  let rec gather st e :=
-    let fcc x :=
-      let v := gather_args st in
-      refl_app v e
-    in
-    let scc _ := st in
-    refl_const scc fcc e
-  with gather_args st F Typs Ft As :=
-    match As with
-      | tt => 
-        let st' := set_add' st F in
-        st'
-      | ( ?A , ?As ) => 
-        match Ft with
-          | ?T1 -> ?T2 =>
-            let Typs' := constr:(Typs ++ (T1:Type) :: @nil Type) in
-            let st' := gather st A in
-            gather_args st' F Typs' T2 As
-          | forall x : ?T1, @?T2 x =>
-            let Ft' := eval simpl in (T2 A) in
-            let F'' := eval simpl in (apply_ls Typs T1 T2 A F) in
-            gather_args st F'' Typs Ft' As
-         end
-    end
+  let cc _ Ts args :=
+    let Ts := eval simpl app in Ts in
+    extend_all_types Ts types
   in
-  let st := constr:((Ts, Ss, Sv)) in
-  let r := gather st exp in
-  r.
+  refl_app cc e. 
 
-Ltac reflect_state refl_const RS RD exp :=
-  let Ts := eval simpl in (Typs RS) in
-  let Ss := eval simpl in (Sym_type RS) in
-  let Sv := eval simpl in (Sym_denote RD) in
-  let E := gather_symbols refl_const Ts Ss Sv exp in
-  match E with
-    | ( ?Ts , ?Ss , ?Sv ) =>
-      let constsOf := eval simpl in (constsOf RS) in
-      let rs := constr:({| Typs       := Ts 
-                         ; constsOf   := constsOf
-                         ; Sym_type   := Ss
-                         |}) in
-      let RS := fresh "RS" in
-      pose (RS := rs) ;
-      let constIn := eval simpl in (constIn RD) in
-      let rd := constr:(Build_ReflDenote RS constIn Sv) in
-      let RD := fresh "RD" in
-      pose (RD := rd) ;
-      let Vs := constr:(@nil nat) in
-      let Vv := constr:(tt) in
-      let r := reflect_expr refl_const RS Ts Ss Sv Vs Vv exp in
-      let r' := r in
-      pose r'
-  end.
+(*
+Ltac buildFuncs types e funcs :=
+  let cc f Ts args :=
+    
+  refl_app cc e 
 
-Goal (nat -> nat) -> (nat -> Prop) -> True.
-intros H P.
+Goal forall a b : nat, a + b = b + a.
+  intros. Set Printing Implicit.
   match goal with
-    | [ |- _ ] =>
-      let exp := constr:(@eq nat (H 1) 1) in
-      reflect_state refl_nat_const ReflSpine_nat ReflDenote_nat exp
+    | [ |- ?G ] =>
+      let ls := constr:(@nil type) in
+      let ts := buildTypes G ls in
+      idtac ts
   end.
-trivial.
-Qed.
+
+Ltac inList x ls :=
+  match ls with
+    | nil => false
+    | x :: _ => true
+    | _ :: ?ls' => inList x ls'
+  end.
+
+Ltac extend x ls :=
+  let b := inList x ls in
+    match b with
+      | true => ls
+      | _ => constr:(x :: ls)
+    end.
+
+
+
+
+
+Ltac buildTypes e types :=
+  match e with
+    | ?f ?a ?b ?c => match type of f with
+                       | ?D1 -> ?D2 -> ?D3 -> ?R =>
+                         let types := extend_type (defaultType D1) types in
+                         let types := extend_type (defaultType D2) types in
+                         let types := extend_type (defaultType D3) types in
+                         let types := extend_type (defaultType R) types in
+                         let types := buildTypes a types in
+                         let types := buildTypes b types in
+                           buildTypes c types
+                       | _ =>
+                         match type of (f a) with
+                           | ?D1 -> ?D2 -> ?R =>
+                             let types := extend (defaultType D1) types in
+                             let types := extend (defaultType D2) types in
+                             let types := extend (defaultType R) types in
+                             let types := buildTypes b types in
+                               buildTypes c (defaultType Empty_set) types
+                         end
+                     end
+    | ?f ?a ?b => match type of f with
+                    | ?D1 -> ?D2 -> ?R =>
+                      let types := extend (defaultType D1) types in
+                      let types := extend (defaultType D2) types in
+                      let types := extend (defaultType R) types in
+                      let types := buildTypes a types in
+                        buildTypes b types
+                    | _ =>
+                      match type of (f a) with
+                        | ?D1 -> ?R =>
+                          let types := extend (defaultType D1) types in
+                          let types := extend (defaultType R) types in
+                            buildTypes b types
+                      end
+                  end
+    | ?f ?a => match type of f with
+                 | ?D1 -> ?R =>
+                   let types := extend (defaultType D1) types in
+                   let types := extend (defaultType R) types in
+                     buildTypes a types
+               end
+    | _ => types
+  end.
+
+Ltac indexOf x ls :=
+  match ls with
+    | x :: ?ls' => constr:(FO (length ls'))
+    | _ :: ?ls' => let f := indexOf x ls' in constr:(FS f)
+  end.
+
+Definition default t (ts : list type) : signature (t :: ts) :=
+  Build_signature (types := t :: ts) (Some (FO _) :: nil) (Some (FO _)) (fun x => x).
+
+Ltac buildFuncs e types types' funcs :=
+  match e with
+    | ?f ?a ?b ?c => match type of f with
+                       | ?D1 -> ?D2 -> ?D3 -> ?R =>
+                         let D1 := indexOf D1 types' in
+                         let D2 := indexOf D2 types' in
+                         let D3 := indexOf D3 types' in
+                         let R := indexOf R types' in
+                         let funcs := extend (Build_signature (types := types) (D1 :: D2 :: D3 :: nil) R f) funcs in
+                           buildFuncs a types types' funcs
+                       | _ => match type of (f a) with
+                                | ?D1 -> ?D2 -> ?R =>
+                                  let D1 := indexOf D1 types' in
+                                  let D2 := indexOf D2 types' in
+                                  let R := indexOf R types' in
+                                  let funcs := extend (Build_signature (types := types) (D1 :: D2 :: nil) R f) funcs in
+                                    buildFuncs a types types' funcs
+                              end 
+                     end
+    | ?f ?a ?b => match type of f with
+                    | ?D1 -> ?D2 -> ?R =>
+                      let D1 := indexOf D1 types' in
+                      let D2 := indexOf D2 types' in
+                      let R := indexOf R types' in
+                      let funcs := extend (Build_signature (types := types) (D1 :: D2 :: nil) R f) funcs in
+                        buildFuncs a types types' funcs
+                    | _ => match type of (f a) with
+                             | ?D1 -> ?R =>
+                               let D1 := indexOf D1 types' in
+                               let R := indexOf R types' in
+                               let funcs := extend (Build_signature (types := types) (D1 :: nil) R f) funcs in
+                                 buildFuncs a types types' funcs
+                           end
+                  end
+    | ?f ?a => match type of f with
+                 | ?D1 -> ?R =>
+                   let D1 := indexOf D1 types' in
+                   let R := indexOf R types' in
+                   let funcs := extend (Build_signature (types := types) (D1 :: nil) R f) funcs in
+                     buildFuncs a types types' funcs
+               end
+    | _ => funcs
+  end.
+
+Ltac indexOfF x ls :=
+  match ls with
+    | Build_signature _ _ x :: ?ls' => constr:(FO (length ls'))
+    | _ :: ?ls' => let f := indexOfF x ls' in constr:(FS f)
+  end.
+
+Ltac buildVars isConst types types' funcs e vars :=
+  match e with
+    | ?f ?a =>
+      let f := indexOfF f funcs in
+        buildVars isConst types types' funcs a vars
+    | ?f ?a ?b =>
+      let f := indexOfF f funcs in
+      let vars := buildVars isConst types types' funcs a vars in
+        buildVars isConst types types' funcs b vars
+    | ?f ?a ?b =>
+      let f := indexOfF (f a) funcs in
+        buildVars isConst types types' funcs b vars
+    | ?f ?a ?b ?c =>
+      let f := indexOfF f funcs in
+      let vars := buildVars isConst types types' funcs a vars in
+      let vars := buildVars isConst types types' funcs b vars in
+        buildVars isConst types types' funcs c vars
+    | ?f ?a ?b ?c =>
+      let f := indexOfF (f a) funcs in
+      let vars := buildVars isConst types types' funcs b vars in
+        buildVars isConst types types' funcs c vars
+    | _ =>
+      match isConst e with
+        | true => vars
+        | _ =>
+          let t := type of e in
+          let t := indexOf t types' in
+          extend (Build_variable (types := types) t e) vars
+      end
+  end.
+
+Ltac indexOfV x ls :=
+  match ls with
+    | Build_variable _ x :: ?ls' => constr:(FO (length ls'))
+    | _ :: ?ls' => let f := indexOfV x ls' in constr:(FS f)
+  end.
+
+Ltac buildExpr isConst types types' funcs vars e :=
+  match e with
+    | ?f ?a =>
+      let f := indexOfF f funcs in
+      let a := buildExpr isConst types types' funcs vars a in
+        constr:(Func (types := types) (funcs := funcs) (vars := vars) f (HCons a HNil))
+    | ?f ?a ?b =>
+      let f := indexOfF f funcs in
+      let a := buildExpr isConst types types' funcs vars a in
+      let b := buildExpr isConst types types' funcs vars b in
+        constr:(Func (types := types) (funcs := funcs) (vars := vars) f (HCons a (HCons b HNil)))
+    | ?f ?a ?b =>
+      let f := indexOfF (f a) funcs in
+      let b := buildExpr isConst types types' funcs vars b in
+        constr:(Func (types := types) (funcs := funcs) (vars := vars) f (HCons b HNil))
+    | ?f ?a ?b ?c =>
+      let f := indexOfF f funcs in
+      let a := buildExpr isConst types types' funcs vars a in
+      let b := buildExpr isConst types types' funcs vars b in
+      let c := buildExpr isConst types types' funcs vars c in
+        constr:(Func (types := types) (funcs := funcs) (vars := vars) f (HCons a (HCons b (HCons c HNil))))
+    | ?f ?a ?b ?c =>
+      let f := indexOfF (f a) funcs in
+      let b := buildExpr isConst types types' funcs vars b in
+      let c := buildExpr isConst types types' funcs vars c in
+        constr:(Func (types := types) (funcs := funcs) (vars := vars) f (HCons b (HCons c HNil)))
+    | _ =>
+      match isConst e with
+        | false =>
+          let t := type of e in
+            let t := indexOfV e vars in
+              constr:(Var (types := types) funcs (vars := vars) t)
+        | true =>
+          let t := type of e in
+            let t := indexOf t types' in
+              constr:(Const (types := types) funcs vars t e)
+      end
+  end.
+
+Ltac reflect isConst := intros;
+  match goal with
+    | [ |- ?G ] =>
+      let types := buildTypes G (@nil type) in
+        let types' := eval simpl in (map Impl types) in
+          let funcs := buildFuncs G types types' (@nil (signature types)) in
+            let funcs := eval simpl in funcs in
+              let vars := buildVars isConst types types' funcs G (@nil (variable types)) in
+                let e := buildExpr isConst types types' funcs vars G in
+                  change (exprD e)
+  end.
+
+Ltac consts e :=
+  match e with
+    | true => true
+    | false => true
+    | O => true
+    | S ?n => consts n
+    | _ => false
+  end.
+
+Theorem test1 : negb false = true.
+  reflect consts.
+Abort.
+
+Theorem test2 : forall n m, n + m = m + 0 + n.
+  reflect consts. simpl length.
+Abort.
+*)
