src/Env.v
@@ -1,0 +1,155 @@
+Require Import List Eqdep_dec.
+
+Set Implicit Arguments.
+
+Inductive fin : nat -> Type :=
+| FO : forall n, fin (S n)
+| FS : forall n, fin n -> fin (S n).
+
+Definition finOut n (f : fin n) : match n return fin n -> Type with
+                                    | O => fun _ => Empty_set
+                                    | S n' => fun f => {f' : _ | f = FS f'} + {f = FO _}
+                                  end f :=
+  match f with
+    | FO _ => inright _ (refl_equal _)
+    | FS _ f' => inleft _ (exist _ f' (refl_equal _))
+  end.
+
+Definition finArg n (f : fin n) : option (fin (pred n)) :=
+  match f with
+    | FO _ => None
+    | FS _ f' => Some f'
+  end.
+
+Lemma fin_inj : forall n (x y : fin n),
+  x <> y
+  -> FS x <> FS y.
+  red; intros.
+  assert (finArg (FS x) = finArg (FS y)) by congruence.
+  simpl in *; congruence.
+Qed.
+
+Hint Immediate fin_inj.
+
+Definition finEq : forall n (x y : fin n), {x = y} + {x <> y}.
+  refine (fix finEq n : forall x y : fin n, {x = y} + {x <> y} :=
+    match n return forall x y : fin n, {x = y} + {x <> y} with
+      | O => fun x _ => match finOut x with end
+      | S n' => fun x y => match finOut x, finOut y with
+                             | inleft (exist x' _), inleft (exist y' _) => if finEq _ x' y' then left _ _ else right _ _
+                             | inright _, inright _ => left _ _
+                             | _, _ => right _ _
+                           end
+    end); clear finEq; abstract (subst; auto; try congruence;
+      match goal with
+        | [ H : sig _ |- _ ] => destruct H
+      end; subst; discriminate).
+Defined.
+
+Section get.
+  Variable A : Type.
+
+  Fixpoint get (ls : list A) : fin (length ls) -> A :=
+    match ls return fin (length ls) -> A with
+      | nil => fun f => match f in fin N return match N with
+                                                  | O => A
+                                                  | _ => unit
+                                                end with
+                          | FO _ => tt
+                          | FS _ _ => tt
+                        end
+      | x :: ls' => fun f => match f in fin N return match N with
+                                                       | O => Empty_set
+                                                       | S N' => (fin N' -> A) -> A
+                                                     end with
+                               | FO _ => fun _ => x
+                               | FS _ f' => fun get_ls' => get_ls' f'
+                             end (get ls')
+    end.
+End get.
+
+Section hlist.
+  Variable A : Type.
+  Variable B : A -> Type.
+
+  Inductive hlist : list A -> Type :=
+  | HNil : hlist nil
+  | HCons : forall x ls, B x -> hlist ls -> hlist (x :: ls).
+
+  Definition hlist_hd (T : A) (ls : list A) (v : hlist (T :: ls)) : B T :=
+    match v in hlist ls return match ls with
+                                 | nil => unit
+                                 | a :: _ => B a
+                               end with
+      | HNil => tt
+      | HCons _ _ x _ => x 
+    end.
+
+  Definition hlist_tl (T : A) (ls : list A) (v : hlist (T :: ls)) : hlist ls :=
+    match v in hlist ls return match ls with
+                                 | nil => unit
+                                 | _ :: ls => hlist ls
+                               end with
+      | HNil => tt
+      | HCons _ _ _ x => x 
+    end.
+
+  Variable dec : forall x (y z : B x), option (y = z).
+
+  Definition hlistEq : forall x (y z : hlist x), option (y = z).
+    refine (fix hlistEq x (y : hlist x) : forall z : hlist x, option (y = z) :=
+      match y in hlist x return forall z : hlist x, option (y = z) with
+        | HNil => fun z => match z in hlist x return match x return hlist x -> Type with
+                                                       | nil => fun z => option (HNil = z)
+                                                       | _ => fun _ => unit
+                                                     end z with
+                             | HNil => Some _
+                             | _ => tt
+                           end
+        | HCons _ _ v1 y' => fun z => match z in hlist x return match x return hlist x -> Type with
+                                                                  | nil => fun _ => unit
+                                                                  | t :: x' => fun z => forall (v1 : B t) (y' : hlist x'),
+                                                                    (forall v2, option (v1 = v2))
+                                                                    -> (forall z', option (y' = z'))
+                                                                    -> option (HCons v1 y' = z)
+                                                                end z with
+                                        | HNil => tt
+                                        | HCons _ _ v2 z' => fun v1 _ dec' self => if dec' v2 then if self z' then Some _ else None else None
+                                      end v1 y' (dec v1) (hlistEq _ y')
+      end); clear hlistEq; abstract congruence.
+  Defined.
+
+  Definition hlist_get : forall (ls : list A) (i : fin (length ls)) (h : hlist ls), B (get ls i).
+  refine (fix hlist_get (ls : list A) : forall (i : fin (length ls)), hlist ls -> B (get ls i) :=
+    match ls as ls return forall (i : fin (length ls)), hlist ls -> B (get ls i) with
+      | nil => fun f _ => 
+        match f as _ in fin N return match N with 
+                                       | 0 => B (get nil f)
+                                       | _ => unit
+                                     end with
+          | FO _ => tt
+          | FS _ _ => tt
+        end
+      | x :: ls' => fun f : fin (length (x :: ls')) => _
+(*
+        fun z =>
+        match f as f' in fin N return match N with 
+                                            | 0 => Empty_set
+                                            | S N' => forall Heq : N = length (x :: ls'), B x -> hlist ls' -> B (get (x :: ls') match Heq in _ = T return fin T with
+                                                                                                                                  | refl_equal => f'
+                                                                                                                                end)
+                                          end with
+          | FO _ => _
+          | FS _ _ => _ 
+        end _ _ _
+*)
+    end).
+  Require Import Program.
+  dependent destruction f. inversion 1. assumption.
+  inversion 1. simpl. eapply hlist_get. assumption.
+Defined.
+
+End hlist.
+
+Implicit Arguments HNil [A B].
+Implicit Arguments HCons [A B x ls].
